Prove splitting permission lemma for case when it is a pointer permission

src/Lifetime.v
@@ -10,11 +10,16 @@ From Coq Require Import
      FSets.FMaps.
 
 From Heapster Require Import
-     Utils
-     RoseTree.
+     Utils.
+
+From ITree Require Import
+     ITree
+     Events.Exception.
 
 Import ListNotations.
-Open Scope list_scope.
+Import ITreeNotations.
+
+Local Open Scope itree_scope.
 (* end hide *)
 
 (* Lifetime keys *)
@@ -25,13 +30,6 @@ Definition status_lte (s1 s2 : status) : Prop :=
   | finished, current => False
   | _, _ => True
   end.
-
-(* (** [s1] subsumes [s2]: [s1] cannot finish before [s2] *) *)
-(* Definition status_subsumes (s1 s2 : status) : Prop := *)
-(*   match s1, s2 with *)
-(*   | finished, current => False *)
-(*   | _, _ => True *)
-(*   end. *)
 
 Global Instance status_lte_preorder : PreOrder status_lte.
 Proof.
@@ -74,29 +72,6 @@ Qed.
 
 Definition Lifetimes := list status.
 
-(* Definition parent_of (l1 l2 : Lifetime) : Prop := *)
-(*   l1 = l2 \/ *)
-(*     parent l1 l2 = true. *)
-
-(* Global Instance parent_of_trans : Transitive parent_of. *)
-(* Proof. *)
-(*   repeat intro. destruct H, H0; subst; unfold parent_of; auto. *)
-(*   right. eapply parent_trans; eauto. *)
-(* Qed. *)
-
-(* Definition index (l : Lifetime) : nat := *)
-(*   match l with *)
-(*   | node index _ => index *)
-(*   end. *)
-
-(* Definition parents (l : Lifetime) : Parents := *)
-(*   match l with *)
-(*   | node _ parents => parents *)
-(*   end. *)
-
-(* Maybe do a lookup on l for its parents' statuses. This will implicitly end all children lifetimes hwen you end a parent lifetime *)
-
-(* Alternatively make ls a total map, so we can keep track of *all* children *)
 Definition statusOf (l : nat) (ls : Lifetimes) : option status :=
   nth_error ls l.
 
@@ -170,118 +145,26 @@ Proof.
     + cbn.
 Abort. (* not used right now *)
 
-(*
-  Program Definition newLifetime (ls : Lifetimes) (ps : list Lifetime) (H : forall p, In p parents -> inL p ls) :
-    (Lifetime * Lifetimes) :=
-    let i := length (lst ls) in
-    let parentIndices := map index parents in
-    (
-      node i parents,
-      {|
-        lst := lst ls ++ [(current, parentIndices)];
-      |}
-    ).
-  Next Obligation.
-  Admitted.
-  Next Obligation.
-    pose proof parents_subsumption.
-  Admitted.
-  Next Obligation.
-  Admitted.
- *)
+(** * Lifetime Computations *)
+Section LifetimeOps.
+  Context {Si Ss : Type}.
+  Context `{Hlens: Lens Si Lifetimes}.
 
-(*
-Variant Lifetime := current | finished.
+  Definition beginLifetime : itree (sceE Si) nat :=
+    s <- trigger (Modify id);;
+    trigger (Modify (fun s => lput s ((lget s) ++ [current])));;
+    Ret (length (lget s)).
 
-Definition Lifetimes := list Lifetime.
-
-(** lifetime helpers **)
-
-Definition lifetime : Lifetimes -> nat -> option Lifetime :=
-  @nth_error Lifetime.
-
-(* Definition replace_lifetime (l : Lifetimes) (n : nat) (new : Lifetime) : Lifetimes := *)
-(*   replace_list_index l n new. *)
-
-(* Lemma replace_lifetime_same c n l : *)
-(*   lifetime c n = Some l -> replace_lifetime c n l = c. *)
-(* Proof. *)
-(*   apply replace_list_index_eq. *)
-(* Qed. *)
-
-(* Lemma lifetime_replace_lifetime c n l : *)
-(*   lifetime (replace_lifetime c n l) n = Some l. *)
-(* Proof. *)
-(*   apply nth_error_replace_list_index_eq. *)
-(* Qed. *)
-
-(** [n1] in the lifetime list [x1] subsumes [n2] in the lifetime list [x2] *)
-Definition subsumes n1 n2 x1 x2 :=
-  (Some current = lifetime x2 n2 -> Some current = lifetime x1 n1) /\
-  (Some finished = lifetime x1 n1 -> Some finished = lifetime x2 n2) /\
-  (None = lifetime x1 n1 -> None = lifetime x2 n2).
-
-(* TODO: generalize to a single lemma *)
-Instance subsumes_preorder x : PreOrder (fun a b => subsumes a b x x).
-Proof.
-  unfold subsumes.
-  constructor; [repeat intro; auto |].
-  intros n1 n2 n3. intros (? & ? & ?) (? & ? & ?). split; [| split]; intros.
-  - apply H. apply H2; auto.
-  - apply H3. apply H0; auto.
-  - apply H4. apply H1; auto.
-Qed.
-Instance subsumes_preorder' x : PreOrder (subsumes x x).
-Proof.
-  unfold subsumes.
-  constructor; [repeat intro; auto |].
-  intros n1 n2 n3. intros (? & ? & ?) (? & ? & ?). split; [| split]; intros.
-  - apply H. apply H2; auto.
-  - apply H3. apply H0; auto.
-  - apply H4. apply H1; auto.
-Qed.
-
-Lemma subsumes_decidable n1 n2 l1 l2 : decidable (subsumes n1 n2 l1 l2).
-Proof.
-  unfold subsumes.
-Admitted.
-
-Lemma not_subsumes n1 n2 n3 l :
-  ~subsumes n1 n3 l l -> ~subsumes n1 n2 l l \/ ~subsumes n2 n3 l l.
-Proof.
-  intro H. red in H.
-  destruct (lifetime l n1) eqn:Hl1; [destruct l0 |];
-    (destruct (lifetime l n2) eqn:Hl2; [destruct l0 |]);
-    (destruct (lifetime l n3) eqn:Hl3; [destruct l0 |]).
-  all: try solve [exfalso; apply H; split; [| split];
-                  rewrite Hl1, Hl3; auto; intro Hc; discriminate Hc].
-  all: try solve [left; intro H'; red in H'; rewrite Hl1, Hl2 in H';
-                  destruct H' as (H1 & H2 & H3);
-                  try solve [discriminate H1; auto];
-                  try solve [discriminate H2; auto];
-                  try solve [discriminate H3; auto]].
-  all: try solve [right; intro H'; red in H'; rewrite Hl2, Hl3 in H';
-                  destruct H' as (H1 & H2 & H3);
-                  try solve [discriminate H1; auto];
-                  try solve [discriminate H2; auto];
-                  try solve [discriminate H3; auto]].
-Qed.
-
-(** Lifetime ordering **)
-Definition lifetime_lte (l1 l2 : option Lifetime) : Prop :=
-  match l1, l2 with
-  | None, _ => True
-  | Some current, None => False
-  | Some current, _ => True
-  | Some finished, Some finished => True
-  | _, _ => False
-  end.
-
-Instance lifetime_lte_preorder : PreOrder lifetime_lte.
-Proof.
-  constructor; repeat intro.
-  - destruct x as [[] |]; simpl; auto.
-  - destruct x as [[] |], y as [[] |], z as [[] |]; simpl; intuition.
-Qed.
-
-*)
+  Definition endLifetime (l : nat) : itree (sceE Si) unit :=
+    s <- trigger (Modify id);;
+    match nth_error (lget s) l with
+    | Some current =>
+        trigger (Modify (fun s =>
+                           (lput s (replace_list_index
+                                      (lget s)
+                                      l
+                                      finished))));;
+        Ret tt
+    | _ => throw tt
+    end.
+End LifetimeOps.
