src/LifetimeMemoryPerms.v
@@ -1,0 +1,211 @@
+(* begin hide *)
+From Coq Require Import
+     Arith.PeanoNat
+     Logic.FunctionalExtensionality
+     Logic.Decidable
+     Lists.List
+     Lia
+     Classes.RelationClasses
+     Classes.Morphisms
+     FSets.FMaps.
+
+From ITree Require Import
+     ITree
+     Eq.Eqit.
+
+From Heapster Require Import
+     Utils
+     Permissions
+     PermType
+     Memory
+     Lifetime
+     MemoryPerms
+     LifetimePerms
+     Typing
+     SepStep.
+
+From Paco Require Import
+     paco.
+
+Import ListNotations.
+Open Scope list_scope.
+(* end hide *)
+
+Section Perms.
+  Context {Si Ss : Type}.
+  Context `{Hmemory: Lens Si memory}.
+  Context `{Hlifetime: Lens Si Lifetimes}.
+
+  Context `{HGetPut1 : (forall x y, @lget _ _ Hmemory (@lput _ _ Hlifetime x y) = @lget _ _ Hmemory x)}.
+  Context `{HGetPut2 : (forall x y, @lget _ _ Hlifetime (@lput _ _ Hmemory x y) = @lget _ _ Hlifetime x)}.
+  Context `{HPutPut : (forall si x y, @lput _ _ Hmemory (@lput _ _ Hlifetime si x) y =
+                                   @lput _ _ Hlifetime (@lput _ _ Hmemory si y) x)}.
+  (* Context `{HPutPut2 : (forall si x y, @lput _ _ Hlifetime (@lput _ _ Hmemory si x) y = *)
+  (*                                   @lput _ _ Hmemory (@lput _ _ Hlifetime si y) x)}. *)
+
+  Lemma nonLifetime_read_perm p v :
+    @nonLifetime _ Ss _ (read_perm p v).
+  Proof.
+    intros n. split; intros [] [].
+    - intros. cbn in *. destruct H as ((? & H) & _). rewrite H. rewrite HGetPut1. reflexivity.
+    - intros. cbn in *. subst. split; reflexivity.
+  Qed.
+  Lemma nonLifetime_write_perm p v :
+    @nonLifetime _ Ss _ (write_perm p v).
+  Proof.
+    intros n. split; intros [] [].
+    - intros. cbn in *. destruct H as ((? & H) & _). rewrite H. rewrite HGetPut1. reflexivity.
+    - intros. cbn in *. destruct H as ((? & H) & _). rewrite H. do 2 rewrite HGetPut2.
+      split; reflexivity.
+  Qed.
+
+  Lemma guar_inv_read_perm p v :
+    @guar_inv _ Ss _ (read_perm p v).
+  Proof.
+    repeat intro. cbn in *. subst. reflexivity.
+  Qed.
+  Lemma guar_inv_write_perm p v :
+    @guar_inv _ Ss _ (write_perm p v).
+  Proof.
+    repeat intro. destruct H as ((? & ?) & ? & ? & ?). subst.
+    cbn. rewrite !HGetPut1, HGetPut2.
+    split; [| split; [| split]]; auto.
+    eexists. rewrite HPutPut. reflexivity.
+  Qed.
+
+  Lemma nonLifetime_ptr p rw o' :
+    @nonLifetime_Perms _ Ss _ ((VPtr p) :: ptr(rw, o', trueP) ▷ tt).
+  Proof.
+    intros q Hq. destruct p as [b o]. destruct Hq as (? & (v & ?) & ?). subst.
+    destruct H0 as (p & p' & Hp & _ & Hsep & Hlte). destruct rw.
+    - exists (read_perm (b, o + o') v). split; [| split; [| split]].
+      + eexists. split. eexists. reflexivity.
+        cbn. eexists. exists bottom_perm. intuition. reflexivity.
+        apply separate_bottom. rewrite sep_conj_perm_bottom. reflexivity.
+      + etransitivity; eauto. etransitivity; eauto. apply lte_l_sep_conj_perm.
+      + apply nonLifetime_read_perm.
+      + apply guar_inv_read_perm.
+    - exists (write_perm (b, o + o') v). split; [| split; [| split]].
+      + eexists. split. eexists. reflexivity.
+        cbn. eexists. exists bottom_perm. intuition. reflexivity.
+        apply separate_bottom. rewrite sep_conj_perm_bottom. reflexivity.
+      + etransitivity; eauto. etransitivity; eauto. apply lte_l_sep_conj_perm.
+      + apply nonLifetime_write_perm.
+      + apply guar_inv_write_perm.
+  Qed.
+
+  Lemma separate_write_perm p l v v' :
+    p ⊥ @write_perm _ Ss _ l v ->
+    p ⊥ write_perm l v'.
+  Proof.
+    intros H. split; apply H; auto.
+  Qed.
+
+  Lemma sep_step_write_perm p l v v' :
+    sep_step p (@write_perm _ Ss _ l v) ->
+    sep_step p (write_perm l v').
+  Proof.
+    repeat intro. split; apply H; auto.
+  Qed.
+
+  Lemma split_Perms b o l (P Q : @Perms (Si * Ss)) :
+    (VPtr (b, o)) :: ptr(W, 0, trueP) ▷ tt * lowned_Perms' l P Q ⊨
+      when_Perms l ((VPtr (b, o)) :: ptr(W, 0, trueP) ▷ tt) *
+      lowned_Perms' l
+                    (when_Perms l ((VPtr (b, o)) :: ptr(R, 0, trueP) ▷ tt) * P)
+                    (((VPtr (b, o)) :: ptr(W, 0, trueP) ▷ tt) * Q).
+  Proof.
+    intros p0 (p' & powned & Hp' & (r1 & r2 & Hr1 & Hr2 & Hr2' & Hsep' & Hr2'' & Hlte' & Hf) & Hsep & Hlte).
+    destruct (nonLifetime_ptr _ _ _ _ Hp') as (p & Hp & Hpp' & Hnlp & Hguarp).
+    exists (when l p Hnlp).
+    assert (Hpr2 : p ⊥ r2).
+    {
+      eapply owned_sep; auto.
+      eapply separate_antimonotone.
+      2: {
+        etransitivity. apply lte_r_sep_conj_perm. eauto.
+      }
+      symmetry. eapply separate_antimonotone; eauto. symmetry. auto.
+    }
+    eexists (r1 ** owned l (p ** r2) (nonLifetime_sep_conj_perm _ _ Hnlp Hr2 Hpr2)).
+    split; [| split; [| split]]; auto.
+    - apply when_perm_Perms; auto.
+    - exists r1, (p ** r2), Hr1, (nonLifetime_sep_conj_perm _ _ Hnlp Hr2 Hpr2), (guar_inv_sep_conj_perm _ _ Hguarp Hr2').
+      split; [| split; [| split]].
+      3: reflexivity.
+      {
+        apply sep_owned; auto. eapply separate_antimonotone. 2: apply Hpp'.
+        symmetry. eapply separate_antimonotone. apply Hsep.
+        etransitivity; eauto. apply lte_l_sep_conj_perm.
+      }
+      {
+        apply sep_conj_Perms_perm; auto.
+      }
+      intros p1 (pw & q & (? & (pr & Hpr' & Hpr & ?) & Hlte''') & Hq' & Hsep''' & Hlte'') Hsep''; subst.
+      cbn in Hlte'''.
+      specialize (Hf _ Hq'). destruct Hf as (r & Hr & Hsep_step & Hpre).
+      {
+        symmetry in Hsep''.
+        eapply separate_antimonotone in Hsep''; eauto.
+        eapply separate_antimonotone in Hsep''; eauto.
+        2: apply lte_r_sep_conj_perm.
+        symmetry in Hsep''.
+        eapply separate_antimonotone in Hsep''; eauto.
+        apply sep_conj_perm_monotone. reflexivity.
+        apply owned_monotone. apply lte_r_sep_conj_perm.
+      }
+      cbn in Hp.
+      destruct Hp as (? & (v & ?) & Hx). subst. rewrite Nat.add_0_r in Hx.
+      rewrite sep_conj_Perms_commut in Hx. rewrite sep_conj_Perms_bottom_identity in Hx.
+      cbn in Hx.
+
+      destruct Hpr as (? & (v' & ?) & Hx'). subst. rewrite Nat.add_0_r in Hx'.
+      rewrite sep_conj_Perms_commut in Hx'. rewrite sep_conj_Perms_bottom_identity in Hx'.
+      cbn in Hx'.
+      exists ((write_perm (b, o) v') ** r). split; [| split].
+      + apply sep_conj_Perms_perm; auto.
+        * cbn. eexists. split. eexists. reflexivity.
+          rewrite Nat.add_0_r.
+          rewrite sep_conj_Perms_commut. rewrite sep_conj_Perms_bottom_identity.
+          cbn. reflexivity.
+        * symmetry. eapply separate_write_perm.
+          apply Hsep_step.
+          eapply separate_antimonotone.
+          2: apply Hx.
+          symmetry. auto.
+      + etransitivity.
+        * apply sep_step_sep_conj_r; eauto. symmetry. auto.
+        * apply sep_step_sep_conj_l; eauto. symmetry. apply Hsep_step. symmetry. auto.
+          eapply sep_step_write_perm.
+          apply sep_step_lte'; eauto.
+      + intros. split; [| split]; auto.
+        * apply Hlte'' in H. destruct H as (? & ? & ?).
+          apply Hlte''' in H. cbn in H.
+          rewrite lGetPut in H. setoid_rewrite nth_error_replace_list_index_eq in H.
+          apply Hx' in H. cbn in *.
+          rewrite HGetPut1 in H |- *; auto. right. reflexivity.
+        * apply Hpre; auto. apply Hlte''; auto.
+        * symmetry. apply Hsep_step.
+          eapply separate_write_perm.
+          eapply separate_antimonotone. symmetry. apply Hpr2. apply Hx.
+    - apply separate_sep_conj_perm.
+      + apply sep_when; auto.
+        symmetry.
+        eapply separate_antimonotone. 2: apply Hpp'.
+        symmetry.
+        eapply separate_antimonotone. apply Hsep. etransitivity; eauto.
+        apply lte_l_sep_conj_perm.
+      + apply when_owned_sep.
+      + symmetry. apply sep_owned; auto. eapply separate_antimonotone. 2: apply Hpp'.
+        symmetry. eapply separate_antimonotone. apply Hsep.
+        etransitivity; eauto. apply lte_l_sep_conj_perm.
+    - etransitivity; eauto.
+      etransitivity. 2: apply sep_conj_perm_monotone; [reflexivity |].
+      2: apply Hlte'.
+      do 2 rewrite <- sep_conj_perm_assoc.
+      do 2 rewrite (sep_conj_perm_commut _ r1).
+      do 2 rewrite sep_conj_perm_assoc.
+      apply sep_conj_perm_monotone; [reflexivity |].
+      etransitivity. apply convert.
+      apply sep_conj_perm_monotone; [| reflexivity]; auto.
+  Qed.
